composite and range work

range2.bpl
@@ -9,10 +9,10 @@ var fracRange : [Ref] real;
 var packedRange : [Ref] bool;
 var fracUniRange : [Ref] real;
 var packedUniRange : [Ref] bool;
-var paramxRange : [Ref] int;
-var paramyRange : [Ref] int;
-var paramxUniRange : [Ref] int;
-var paramyUniRange : [Ref] int;
+var paramRangeX : [Ref] int;
+var paramRangeY : [Ref] int;
+var paramUniRangeX : [Ref] int;
+var paramUniRangeY : [Ref] int;
 
 
 procedure ConstructLink(x: int, y:int, val1: int, next1: Ref, this: Ref);
@@ -22,6 +22,7 @@ procedure ConstructLink(x: int, y:int, val1: int, next1: Ref, this: Ref);
 procedure PackRange(x:int, y:int, this:Ref);
 	requires (val[this] >= x);
 	requires (val[this] <= y);
+  requires (next[this] != this);
 	requires ((next[this] == null) ||
 		  (fracRange[next[this]] > 0.0)
 	 );
@@ -34,47 +35,54 @@ procedure UnpackRange(x:int, y:int, this:Ref);
 		 ((next[this] == null) ||
 		  (fracRange[next[this]] > 0.0) 
 		 );
+  ensures (next[this] != this);
 
 procedure PackUniRange(x:int, y:int, this:Ref);
 	requires (val[this] >= x);
 	requires (val[this] <= y);
+  requires (next[this] != this);
 	requires ((next[this] == null) ||
 		(
 		(fracUniRange[next[this]] == 1.0) &&
-    		packedUniRange[next[this]] &&
-		(paramxUniRange[next[this]] == x) &&
-		(paramyUniRange[next[this]] == y)
+    		packedUniRange[next[this]] 
 		)
 );
 
 procedure UnpackUniRange(x:int, y:int, this:Ref);
 	requires packedUniRange[this];
 	requires (fracUniRange[this] > 0.0);
-	requires (paramxUniRange[this] == x);
-	requires (paramyUniRange[this] == y);
+	requires (paramUniRangeX[this] == x);
+	requires (paramUniRangeY[this] == y);
 	ensures  (val[this] >= x) &&
 		 (val[this] <= y) &&
 		 ((next[this] == null) ||
 		((fracUniRange[next[this]] == 1.0) &&
          	packedUniRange[next[this]] &&
-		(paramxUniRange[next[this]] == x) &&
-		(paramyUniRange[next[this]] == y)
+		(paramUniRangeX[next[this]] == x) &&
+		(paramUniRangeY[next[this]] == y)
 ) 
 		 );
+    ensures (next[this] != this);
+	
 
 procedure add(z:int, x:int, y:int, this: Ref)
-	modifies val, packedUniRange, fracUniRange, paramxUniRange, paramyUniRange;
+	modifies val, packedUniRange, fracUniRange, paramUniRangeX, paramUniRangeY;
 	requires x < y;
 	requires fracUniRange[this] == 1.0;
-  	requires packedUniRange[this];
-	requires paramxUniRange[this] == x;
-	requires paramyUniRange[this] == y;
+  requires packedUniRange[this];
+	requires paramUniRangeX[this] == x;
+	requires paramUniRangeY[this] == y;
 	ensures packedUniRange[this];
-	ensures paramxUniRange[this] == x+z;
-	ensures paramyUniRange[this] == y+z;
+	ensures paramUniRangeX[this] == x+z;
+	ensures paramUniRangeY[this] == y+z;
 	ensures packedUniRange[this];
-  	ensures fracUniRange[this] == 1.0;
+  ensures fracUniRange[this] == 1.0;
+  ensures (forall y1:Ref :: (packedUniRange[y1] == old(packedUniRange[y1])) );
+	ensures (forall y1:Ref :: (fracUniRange[y1] == old(fracUniRange[y1])) ); 
+  ensures (forall y1:Ref :: ( ( (next[y1] == this) ==> (paramUniRangeX[y1] == old(paramUniRangeX[y1]))  )  ) );
+  ensures (forall y1:Ref :: ( ( (next[y1] == this) ==> (paramUniRangeY[y1] == old(paramUniRangeY[y1]))  )  ) );
 {
+
 	call UnpackUniRange(x, y, this);
 
 	packedUniRange[this] := false;
@@ -82,57 +90,56 @@ procedure add(z:int, x:int, y:int, this: Ref)
 	val[this] := val[this]+z;
 
 	if (next[this] != null )
-	{ 
-//The assume is better right before the call because
-//there is a rationale for putting it here. 
-//Same for the assume right after the call.
-	assume (this != next[this]);
-    	call add(z, x, y, next[this]);
-    	assume (val[this]==old(val[this])+z);
+	{  
+ 
+    call add(z, x, y, next[this]);
+   
 	}
   
-  	call PackUniRange(x+z, y+z, this);
+    call PackUniRange(x+z, y+z, this);
 	packedUniRange[this] := true;
 	fracUniRange[this] :=  1.0;
-	paramxUniRange[this] := x+z;
-	paramyUniRange[this] := y+z;
+	paramUniRangeX[this] := x+z;
+	paramUniRangeY[this] := y+z;
+
 
 }
 
 procedure addModulo11(x:int, this: Ref) 
-	modifies val, packedRange, fracRange, paramxRange, paramyRange;
+	modifies val, packedRange, fracRange, paramRangeX, paramRangeY;
 	requires x >= 0;
 	requires fracRange[this] > 0.0;
-	requires paramxRange[this] == 0;
-	requires paramyRange[this] == 10;
-  	requires (forall y:Ref :: (packedRange[y] == true));
+	requires paramRangeX[this] == 0;
+	requires paramRangeY[this] == 10;
+  requires (forall y:Ref :: packedRange[y]);
+	requires (forall y:Ref :: paramRangeX[y] == 0);
+	requires (forall y:Ref :: paramRangeY[y] == 10);
 	ensures packedRange[this];
-	ensures paramxRange[this] == 0;
-	ensures paramyRange[this] == 10;
 	ensures fracRange[this] > 0.0;
 	ensures (forall y:Ref :: (packedRange[y] == old(packedRange[y])) );
+  ensures (forall y:Ref :: (paramRangeX[y] == old(paramRangeX[y])) );
 	ensures (forall y:Ref :: (fracRange[y] == old(fracRange[y])) );
+  ensures (forall y:Ref :: (paramRangeX[y] == old(paramRangeX[y])) );
 {
 	call UnpackRange(0, 10, this);
 	packedRange[this] := false;
 	fracRange[next[this]] := fracRange[next[this]] * 2.0;
 
 	val[this] := modulo((val[this]+x),11);
-  
-  	call PackRange(0, 10, this);
+
+	call PackRange(0, 10, this);
 	packedRange[this] := true;
-	paramxRange[this] := 0;
-	paramyRange[this] := 10;
+	paramRangeX[this] := 0;
+	paramRangeY[this] := 10;
 	fracRange[next[this]] := fracRange[next[this]] / 2.0;
-	paramxRange[this] := 0;
 	
 	if (next[this] != null )
 	{ 
-    
 		call addModulo11(x, next[this]);
 		fracRange[next[this]] := fracRange[next[this]] * 2.0;
 		fracRange[next[this]] := fracRange[next[this]] / 2.0;
 	}
+     
 }
 
 function modulo(x:int, y:int) returns (int);
@@ -148,7 +155,9 @@ axiom (forall x:int, y:int :: {modulo(x,y)}
 
 
 procedure main()
-	modifies val, packedRange, fracRange, paramxRange, paramyRange;
+	modifies val, packedRange, fracRange, paramRangeX, paramRangeY;
+	requires (forall y:Ref :: paramRangeX[y] == 0);
+	requires (forall y:Ref :: paramRangeY[y] == 10);
    requires (forall y:Ref :: (packedRange[y] == true));
 {
 	var l1 : Ref;
@@ -157,23 +166,23 @@ procedure main()
 	call ConstructLink(0, 10, 3, null, l1);
 	packedRange[l1] := true;
 	fracRange[l1] := 1.0;
-	paramxRange[l1] := 0;
-	paramyRange[l1] := 10;
+	paramRangeX[l1] := 0;
+	paramRangeY[l1] := 10;
 
 
 	call ConstructLink(0, 10, 4, l1, l2);
 	fracRange[l1] := fracRange[l1] / 2.0;
 	packedRange[l2] := true;
 	fracRange[l2] := 1.0;
-	paramxRange[l2] := 0;
-	paramyRange[l2] := 10;
+	paramRangeX[l2] := 0;
+	paramRangeY[l2] := 10;
 
 	call ConstructLink(0, 10, 5, l2, l3);
 	fracRange[l2] := fracRange[l2] / 2.0;
 	packedRange[l3] := true;
 	fracRange[l3] := 1.0;
-	paramxRange[l3] := 0;
-	paramyRange[l3] := 10;
+	paramRangeX[l3] := 0;
+	paramRangeY[l3] := 10;
 
 	call addModulo11(20, l3); 
 }
